%% -*- coding: utf-8 -*-
\documentclass[pdftex,aspectratio=169]{beamer}

\input{common}
%%% frontmatter
\input{frontmatter}
\subtitle
{Lambda Calculus}

\begin{document}

\begin{frame}
  \titlepage
\end{frame}

%\begin{frame}
%  \frametitle{Outline}
%  \tableofcontents
  % You might wish to add the option [pausesections]
%\end{frame}


\begin{frame}[fragile]
  \frametitle{The Lambda Calculus}
\begin{block}<+->{What Wikipedia says}
  \href{https://en.wikipedia.org/wiki/Lambda_calculus}{Lambda
    calculus} (also written as λ-calculus) is a formal system in
  mathematical logic for expressing computation based on function
  abstraction and application [\dots]. It is a universal model of
  computation that can be used to simulate any Turing machine and was
  first introduced by mathematician Alonzo Church in the 1930s as part
  of his research [on] the foundations of mathematics.  
\end{block}
\begin{block}<+->{Further down it says}
  \begin{itemize}
  \item[\textcolor{green}\cmark] Lambda calculus has applications in many different areas in mathematics, philosophy, linguistics, and computer science.
  \item[\textcolor{green}\cmark] Lambda calculus has played an important role in the development of the theory of programming languages.
  \item[\textcolor{red}\xmark] Functional programming languages implement the lambda calculus.
  % \item Lambda calculus also is a current research topic in Category theory.
  \end{itemize}
\end{block}
\end{frame}             

\begin{frame}[fragile]
  \frametitle{Syntax of the λ-calculus}
  \begin{block}<+->{λ terms}
    \begin{align*}
      M,N & ::= x & \text{variable} \\
          & \mid (\lambda x. M) & \text{(lambda) abstraction} \\
          & \mid (M\, N) & \text{application}
    \end{align*}
    \begin{itemize}
    \item Variables are drawn from infinite denumerable set
    \item $(\lambda x. M)$ \textbf{binds} $x$ in $M$
    \end{itemize}
  \end{block}
  \begin{block}<+->{Conventions for omitting parentheses}
    \begin{itemize}
    \item abstractions extend as far to the right as possible
    \item application is left associative
    \end{itemize}
  \end{block}
\end{frame}             

\begin{frame}[fragile]
  \frametitle{Working with lambda terms}
  \begin{block}{Free and bound variables}
    \begin{align*}
    \free(x) & = \{ x \} \\
    \free(M\,N) & = \free(M) \cup \free(N) \\
    \free(\lambda x.M) & = \free(M) \setminus \{x\}\\[1ex]
    \bound(x) & = \varnothing\\
    \bound(M\,N) & = \bound(M) \cup \bound(N) \\
      \bound(\lambda x.M) & = \bound(M) \cup \{x\} \\[1ex]
      \var (M) & = \free (M) \cup \bound (M)
    \end{align*}
    A  lambda term $M$ is \textbf{closed} ($M$ is a
    \textbf{combinator}) iff $\free(M)=\varnothing$. \\
    Otherwise the term is
  \textbf{open}. 
  \end{block}
\end{frame}

\begin{frame}[fragile]
  \frametitle{Working with lambda terms}
  \begin{block}{Substitution $M[x\mapsto N]$}
    \vspace{-\baselineskip}
    \begin{alignat*}{2}
    x[x\mapsto N] & = N\\
    y[x\mapsto N] & = y \quad & x\neq y\\
    (\lambda x.M)[x\mapsto N] & := \lambda x.M\\
    (\lambda y.M)[x\mapsto N] & := \lambda y.(M[x\mapsto N])
    \quad & x\neq y, y\not\in\free(N)\\
    (\lambda y.M)[x\mapsto N] & := \lambda y'.(M[y\mapsto y'][x\rightarrow N])
    \quad & x\neq y, y\in\free(N), y'\not\in\free(M)\cup\free(N)\\
    (M\,M')[x\mapsto N] & := (M[x\mapsto N])(M'[x\mapsto N])
  \end{alignat*}
\end{block}
\begin{alertblock}{Guiding principle: \textbf{capture freedom}}
  In every $(\lambda x.M)$ the bound variable $x$ is ``connected'' to each
  free occurrence of $x$ in $M$. These connections must not be broken by
  substitution. 
\end{alertblock}
\end{frame}             


\begin{frame}[fragile]
  \frametitle{Computing with lambda terms}
  \begin{block}<+->{Reduction rules}\VSPBLS
    \begin{alignat*}{2}
      (\lambda x.M) & \rightarrow_{\alpha} (\lambda y.M[x\mapsto y]) \quad 
      & y\not\in\free(M) & \quad\text{Alpha reduction (\textcolor{red}{renaming bound
      variables})}
      \\
      ((\lambda x.M)\,N) & \rightarrow_{\beta} M[x\mapsto N]
      && \quad\text{Beta reduction (\textcolor{red}{function application})}
      \\
      (\lambda x.(M\,x)) & \rightarrow_{\eta} M \quad
      & x\not\in\free(M) & \quad \text{Eta reduction}
    \end{alignat*}
    Left hand side of a rule: \textbf{redex}; right hand side: \textbf{contractum}
  \end{block}
  \begin{block}<+->{Reductions may be applied anywhere in a term}
    \begin{displaymath}
    \begin{array}{c}
      M \rightarrow_x M'
      \\\hline
      (\lambda y.M) \rightarrow_x (\lambda y.M')
    \end{array}
    \qquad
    \begin{array}{c}
      M \rightarrow_x M'
      \\\hline
      (M~N) \rightarrow_x (M'~N)
    \end{array}
    \qquad
    \begin{array}{c}
      N \rightarrow_x N'
      \\\hline
      (M~N) \rightarrow_x (M~N')
    \end{array}
  \end{displaymath}
  \end{block}
\end{frame}

\begin{frame}[fragile]
  \frametitle{The theory of the lambda calculus}
  \begin{alertblock}<+->{Computation and equivalence}
    For $x\subseteq\{\alpha,\beta,\gamma\}$ and reduction relation $\rightarrow_x$,
    \begin{itemize}
    \item $\stackrel{\ast}{\rightarrow}_x$ is the reflexive-transitive
      closure,
    \item $\leftrightarrow_x$ is its symmetric closure,
    \item $\overset{\ast}{\leftrightarrow}_x$ is its
      reflexive-transitive-symmetric closure.
    \end{itemize}
  \end{alertblock}
  \begin{alertblock}<+->{Equality in lambda calculus}
    \begin{itemize}
    \item Alpha equivalence: $M =_\alpha N$ iff $M
      \overset{\ast}{\leftrightarrow}_{\alpha} N$.
    \item Standard: $M =_\beta N$ iff $M
      \overset{\ast}{\leftrightarrow}_{\alpha,\beta} N$.
    \item Extensional: $M =_{\beta\eta} N$ iff $M
      \overset{\ast}{\leftrightarrow}_{\alpha,\beta,\eta} N$.
    \end{itemize}
  \end{alertblock}
\end{frame}             


\begin{frame}[fragile]
  \frametitle{Computing with lambda terms}
  \begin{alertblock}<+->{Definition: Normal form}
    Let $M$ be a lambda term. \\
    A lambda term $N$ is a \textbf{normal
      form} of $M$ iff $M\overset{\ast}{\rightarrow}_\beta N$ and there
    is no $N'$ with $N\rightarrow_\beta N'$.
  \end{alertblock}
  \begin{block}<+->{}
    Lambda terms with equivalent (equal modulo $\alpha$ reduction) normal
    forms exhibit the same behavior.
    The reverse is not always true.
  \end{block}
  \begin{alertblock}<+->{A lambda term without normal form}
    \begin{displaymath}
  (\lambda x.x~x)(\lambda x.x~x) \rightarrow_\beta (\lambda
  x.x~x)(\lambda x.x~x) 
\end{displaymath}
  \end{alertblock}
\end{frame}             

\begin{frame}[fragile]
  \frametitle{Computing with lambda terms makes sense}
  \begin{alertblock}<+->{The Church-Rosser theorem}
    Beta reduction has the \textbf{Church-Rosser property}:
    \begin{center}
      \begin{tikzpicture}[scale=0.6,shorten >=1pt, auto]
        \node (M1) at (2,5) {$M_1$} ;
        \node (M2) at (6,5) {$M_2$} ;
        \node (N) at (4,2) {$N$} ;
        \draw
        (M1) edge[<->,thick] node {$\beta\ast$} (M2)
        (N) edge[<-, thick] node {$\beta\ast$} (M1)
        (M2) edge[->, thick] node {$\beta\ast$} (N)
        ;
      \end{tikzpicture}
    \end{center}
    That is: For
    all $M_1, M_2$ with
  $M_1 \overset{\ast}{\leftrightarrow}_\beta M_2$,
  there is some $N$ with
  $M_1\overset{\ast}{\rightarrow}_\beta N$ and
  $M_2\overset{\ast}{\rightarrow}_\beta N$.
\end{alertblock}
\begin{block}<+->{Corollary}
  A lambda term $M$ has at most one normal form modulo $\alpha$
  reduction.
\end{block}
\end{frame}


\begin{frame}[fragile]
  \Huge
  \begin{center}
    {Programming in the pure lambda calculus}
  \end{center}
\end{frame}



\begin{frame}[fragile]
  \frametitle{From functions to arbitrary datatypes}
  \begin{block}{Any computation may be encoded in the lambda calculus}
    \begin{itemize}
    \item Booleans and conditionals
    \item Numbers
    \item Recursion
    \item Products (pairs)
    \item Variants
    \end{itemize}
  \end{block}
\end{frame}             

\begin{frame}[fragile]
  \frametitle{Booleans and conditional}
  \begin{exampleblock}<+->{Requirements / Specification}
    Wanted: Lambda terms $\IF$, $\TRUE$, $\FALSE$ such that
    \begin{itemize}
    \item $\IF~\TRUE~M\,N \stackrel\ast\rightarrow_\beta M$
    \item $\IF~\FALSE~M\,N \stackrel\ast\rightarrow_\beta N$
    \end{itemize}
  \end{exampleblock}
  \begin{exampleblock}<+->{Idea}
    $\TRUE$ and $\FALSE$ are functions that select the first or second
    argument, respectively
  \end{exampleblock}
  \end{frame}

\begin{frame}
  \frametitle{Booleans and conditional}
  \begin{block}<+->{Booleans}\VSPBLS
    \begin{align*}
      \TRUE &= \lambda x.\lambda y.x &
      \FALSE &= \lambda x.\lambda y.y
    \end{align*}
  \end{block}
  \begin{block}<+->{Conditional}\VSPBLS
    \begin{align*}
      \IF &= \lambda b.\lambda t.\lambda f. b\,t\,f
    \end{align*}
  \end{block}
  \begin{alertblock}<+->{Check the spec!}
    \dots
  \end{alertblock}
\end{frame}


\begin{frame}[fragile]
  \frametitle{Natural numbers}
  \begin{exampleblock}{Requirements / Specification}
    Wanted: A family of lambda terms $\lceil n\rceil$, for each
    $n\in\nat$, such that the arithmetic operations are \emph{lambda
      definable}.

    That is, there are lambda terms $\ADD$, $\SUB$, $\MULT$, $\DIV$ such that
    \begin{itemize}
    \item $\ADD~\Encode m~\Encode n \Reduce \Encode{m+n}$
    \item $\SUB~\Encode m~\Encode n \Reduce \Encode{m-n}$
    \item $\MULT~\Encode m~\Encode n \Reduce \Encode{mn}$
    \item $\DIV~\Encode m~\Encode n \Reduce \Encode{m/n}$
    \end{itemize}
  \end{exampleblock}
\end{frame}

\begin{frame}[fragile]
  \frametitle{Church numerals}
\begin{exampleblock}<+->{One approach}
  % Numbers can be represented in several different ways by lambda
  % terms.  One is to use \textbf{Church numerals}.
  The \textbf{Church numeral}
  $\Encode{ n}$ of some natural number $n$ is a function that takes
  two parameters, a function $f$ and some $x$, and applies $f$ $n$-times to $x$.
\end{exampleblock}
\begin{alertblock}<+->{Zero}\VSPBLS
  \begin{align*}
    \Encode{0} & = \lambda f. \lambda x. x
  \end{align*}
\end{alertblock}
\begin{alertblock}<+->{Successor}\VSPBLS
  \begin{align*}
    \SUCC & = \lambda n. \lambda f. \lambda x. f (n\, f\,x)
  \end{align*}
\end{alertblock}
\end{frame}

\begin{frame}[fragile]
  \frametitle{Church numerals --- addition and multiplication}
\begin{alertblock}<+->{Addition}\VSPBLS
  \begin{align*}
    \ADD & = \lambda m. \lambda n. \lambda f. \lambda x. m\, f (n\, f\, x)
  \end{align*}
\end{alertblock}
\begin{alertblock}<+->{Multiplication}\VSPBLS
  \begin{align*}
    \MULT & = \lambda m . \lambda n. \lambda f. \lambda x. m\, (n\, f)\, x
  \end{align*}
\end{alertblock}
\end{frame}

\begin{frame}[fragile]
  \frametitle{Church numerals --- conditional}
  \begin{exampleblock}<+->{Wanted}
    $\IFZ$ such that
    \begin{itemize}
    \item $\IFZ~\Encode 0~M~N \Reduce M$
    \item $\IFZ~\Encode n~M~N \Reduce N$ if $n\ne 0$
    \end{itemize}
  \end{exampleblock}
  \begin{alertblock}<+->{Testing for zero}\VSPBLS
    \begin{align*}
      \IFZ &= \lambda n. \lambda z. \lambda s. n\,(\lambda x. s)\,z
    \end{align*}
  \end{alertblock}
  \begin{alertblock}<+->{Check the spec!}
    \dots
  \end{alertblock}
\end{frame}




\begin{frame}
  \frametitle{Pairs}
  \begin{exampleblock}<+->{Specification}
    Wanted: lambda terms $\PAIR$, $\FST$, $\SND$ such that
    \begin{itemize}
    \item $\FST (\PAIR~M~N) \Reduce M$
    \item $\SND (\PAIR~M~N) \Reduce N$
    \end{itemize}
  \end{exampleblock}
  \begin{alertblock}<+->{Implementation}\VSPBLS
    \begin{align*}
      \PAIR &= \lambda x.\lambda y. \lambda v. v\,x\,y \\
      \FST  &= \lambda p. p (\lambda x.\lambda y. x) \\
      \SND  &= \lambda p. p (\lambda x.\lambda y. y)
    \end{align*}
  \end{alertblock}
\end{frame}

\begin{frame}
  \frametitle{Variants (data Either a b = Left a $\mid$ Right b)}
  \begin{exampleblock}<+->{Specification}
    Wanted: lambda terms $\LEFT$, $\RIGHT$, $\CASE$ such that
    \begin{itemize}
    \item $\CASE (\LEFT~M) N_l\,N_r \Reduce N_l\,M$
    \item $\CASE (\RIGHT~M) N_l\,N_r \Reduce N_r\,M$
    \end{itemize}
  \end{exampleblock}
  \begin{alertblock}<+->{Implementation}\VSPBLS
    \begin{align*}
      \CASE &= \\
      \LEFT &= \\
      \RIGHT&=
    \end{align*}
  \end{alertblock}
\end{frame}

\begin{frame}
  \frametitle{Constructor and case for Haskell data}
  \begin{block}{Scott encoding of data types}
    Suppose a datatype $D$ is defined with constructors
    $K_1, \dots, K_m$ where constructor $j$ takes $n_j$ arguments.
    \begin{align*}
      \Encode{K_j} &= \lambda x_1 \dots x_{n_j}. \lambda c_1 \dots
                     c_m. c_j x_1 \dots x_{n_j}
      \\
      \CASE_D &= \lambda v. \lambda c_1 \dots c_m. v c_1 \dots c_m
      \\
                   &=_\eta \lambda v.v
    \end{align*}
    That is, the encoding of the constructor \textbf{is} the $\CASE_D$
    operation.
    \begin{itemize}
    \item Pair is the special case with one constructor and two
      arguments
    \item Either is the special case with two constructors of one
      argument each
    \end{itemize}
  \end{block}
\end{frame}

\begin{frame}[fragile]
  \frametitle{Scott encoding for natural numbers}
  \begin{block}<+->{Scott numerals $\ne$ Church numerals}
\begin{lstlisting}
data Nat = Zero | Succ Nat
\end{lstlisting}
    \begin{itemize}
    \item Two constructors with arities $0$ and $1$.
    \end{itemize}
    \begin{align*}
      \Encode{\mathtt{Zero}} & = \lambda z\ s. z \\
      \Encode{\mathtt{Succ}} &= \lambda x_1. \lambda z\ s. s\ x_1 \\
      \CASE_{\mathtt{Nat}} &= \lambda v.v
    \end{align*}
  \end{block}
  \begin{block}<+->{Addition with Scott numerals requires fixed point}
    \begin{itemize}
    \item The Church encoding of a datatype represents a value as the
      fold operation over the value.
    \item The Scott encoding represents a value as its case operation.
    \end{itemize}
  \end{block}
\end{frame}

\begin{frame}
  \frametitle{Recursion}
  \begin{alertblock}<+->{Fixed point theorem (see Barendregt, The Lambda Calculus)}
    Every lambda term has a fixed point:

    For every $M$ there is some $N$ such that
    $
    M\, N \overset{\ast}{\leftrightarrow}_\beta N
    $.
  \end{alertblock}
  \begin{exampleblock}<+->{Proof}
    Let $N = Y~M$ where
    \begin{displaymath}
      Y := \lambda f.(\lambda x.f~(x~x))~(\lambda x.f~(x~x)).
    \end{displaymath}
  \end{exampleblock}
  \begin{block}<+->{Remark}
    $Y$ is Curry's \textbf{fixed point combinator}. There are infinitely
    many more fixed point combinators with various properties.
  \end{block}
\end{frame}
\begin{frame}
  \frametitle{Addition with Scott encoding}
  \begin{block}<+->{Definition of addition}
    \vspace{-\baselineskip}
    \begin{align*}
      f_a &= \lambda a. \lambda m\ n. \CASE_{\mathtt{Nat}}\ m\ n\
            (\lambda m'. \Encode{\mathtt{Succ}}\ (a\ m'\ n)) \\
      \Encode{\mathtt{add}} &= Y\  f_a \\
          &= f_a (Y\ f_a) = f_a \Encode{\mathtt{add}}
    \end{align*}
  \end{block}
\end{frame}
\begin{frame}
  \frametitle{Addition with Scott encoding (2)}
\begin{block}<+->{Case Zero}
    \vspace{-\baselineskip}
    \begin{align*}
      \Encode{\mathtt{add}}\ \Encode{\mathtt{Zero}}\ n
      &= f_a\ \Encode{\mathtt{add}} \ \Encode{\mathtt{Zero}}\ n \\
      &= (\lambda m\ n. \CASE_{\mathtt{Nat}}\ m\ n\
        (\lambda m'. \Encode{\mathtt{Succ}}\ (\Encode{\mathtt{add}}\
        m'\ n)))\ \Encode{\mathtt{Zero}}\ n \\
      &= \CASE_{\mathtt{Nat}}\ \Encode{\mathtt{Zero}}\ n\
        (\lambda m'. \Encode{\mathtt{Succ}}\ (\Encode{\mathtt{add}}\
        m'\ n)) \\
      &= \Encode{\mathtt{Zero}}\ n\
        (\lambda m'. \Encode{\mathtt{Succ}}\ (\Encode{\mathtt{add}}\
        m'\ n)) \\
      &= n
    \end{align*}
  \end{block}
  \begin{block}<+->{Case Succ}
    \vspace{-\baselineskip}
    \begin{align*}
      \Encode{\mathtt{add}}\ (\Encode{\mathtt{Succ}}\ k)\ n
      &= \dots \\
      &= (\Encode{\mathtt{Succ}}\ k)\ n\
        (\lambda m'. \Encode{\mathtt{Succ}}\ (\Encode{\mathtt{add}}\
        m'\ n)) \\
      &=(\lambda m'. \Encode{\mathtt{Succ}}\ (\Encode{\mathtt{add}}\
        m'\ n))\ k  \\
      &= \Encode{\mathtt{Succ}}\ (\Encode{\mathtt{add}}\ k\ n)
    \end{align*}
  \end{block}
\end{frame}
\begin{frame}
  \frametitle{Wrapup}
  \begin{itemize}
  \item Beta reduction is the only computation rule of lambda calculus
  \item It applies anywhere in a lambda term
  \item All datatypes can be expressed in lambda calculus
  \item Lambda calculus is able to express the primitives of the
    theory of partial recursive functions
  \item The theory of partial recursive functions is Turing complete
  \item Hence is the (untyped) lambda calculus
  \end{itemize}
\end{frame}
\end{document}


